\documentclass{beamer}

\title{Unification}
\author{Isaac Elliott}

\begin{document}

\frame{\titlepage}

\begin{frame}
  \frametitle{Solve these equations}

  $$ x = 6 - z $$
  $$ y + 5 = 12 - x $$
  $$ z + y = 5 $$

\end{frame}

\begin{frame}
  \frametitle{Solve these equations}

  $$ x = 6 - z $$
  $$ y + 5 = 12 - (6 - z) $$
  $$ z + y = 5 $$

\end{frame}

\begin{frame}
  \frametitle{Solve these equations}

  $$ x = 6 - z $$
  $$ y + 5 = 6 + z $$
  $$ z + y = 5 $$

\end{frame}

\begin{frame}
  \frametitle{Solve these equations}

  $$ x = 6 - z $$
  $$ y = 1 + z $$
  $$ z + y = 5 $$

\end{frame}

\begin{frame}
  \frametitle{Solve these equations}

  $$ x = 6 - z $$
  $$ y = 1 + z $$
  $$ z + (1 + z) = 5 $$

\end{frame}

\begin{frame}
  \frametitle{Solve these equations}

  $$ x = 6 - z $$
  $$ y = 1 + z $$
  $$ z = 2 $$

\end{frame}

\begin{frame}
  \frametitle{Solve these equations}

  $$ x = 6 - 2 $$
  $$ y = 1 + 2 $$
  $$ z = 2 $$

\end{frame}

\begin{frame}
  \frametitle{Solve these equations}

  $$ x = 4 $$
  $$ y = 3 $$
  $$ z = 2 $$

\end{frame}

\begin{frame}
  \frametitle{Solve these equations, round 2}

  $$ x = 2 + y $$
  $$ 3 + y = 2 - z $$
  $$ z + x = 4 $$

\end{frame}

\begin{frame}
  \frametitle{Solve these equations, round 2}

  $$ x = 2 + y $$
  $$ 3 + y = 2 - z $$
  $$ z + (2 + y) = 4 $$

\end{frame}

\begin{frame}
  \frametitle{Solve these equations, round 2}

  $$ x = 2 + y $$
  $$ y = -1 - z $$
  $$ z + (2 + y) = 4 $$

\end{frame}

\begin{frame}
  \frametitle{Solve these equations, round 2}

  $$ x = 2 + (-1 - z) $$
  $$ y = -1 - z $$
  $$ z + (2 + (-1 - z) = 4 $$

\end{frame}

\begin{frame}
  \frametitle{Solve these equations, round 2}

  $$ x = 2 + (-1 - z) $$
  $$ y = -1 - z $$
  $$ z + (1 - z) = 4 $$

\end{frame}

\begin{frame}
  \frametitle{Solve these equations, round 2}

  $$ x = 2 + (-1 - z) $$
  $$ y = -1 - z $$
  $$ 1 = 4 $$

\end{frame}

\begin{frame}
  \frametitle{Solve these equations, round 2}

  Unsolvable!

\end{frame}

\end{document}
